Subtype narrowing

CC/Subtype/Subst.lean
@@ -10,6 +10,7 @@ import CC.Typed
 import CC.Typed.Basic
 import CC.Subtype
 import CC.Subcapt.Subst
+import CC.Narrowing
 
 namespace CC
 
@@ -74,3 +75,11 @@ def Subtype.subst (h : Subtype Γ T1 T2) (σ : VarSubst Γ Δ f) (δ : TVarRenam
   constructor
   apply Subcapt.subst <;> aesop
   apply SubtypeP.subst <;> aesop
+
+def Subtype.narrow_var (hsub : Subtype Γ T1 T2)
+  (h0 : Subtype (Ctx.extend_var Γ T2) U1 U2) :
+  Subtype (Ctx.extend_var Γ T1) U1 U2 := by
+  have h := Subtype.subst h0 (VarSubst.narrowing_var hsub) TVarRename.narrowing_var
+  rw [<- CType.rename_id (T := U1)]
+  rw [<- CType.rename_id (T := U2)]
+  exact h
