CC/Context.lean
@@ -34,3 +34,23 @@ inductive BoundTVar : Ctx n m -> Fin m -> PType n m -> Prop where
 | there_tvar :
   BoundTVar Γ x S ->
   BoundTVar (Ctx.extend_tvar Γ S') x.succ S.weaken_tvar
+
+def BoundVar.pred'
+  {Γ : Ctx n m} {P : CType n m} {T : CType n.succ m} :
+  Γ0 = Ctx.extend_var Γ P ->
+  x0 = x.succ ->
+  BoundVar Γ0 x0 T ->
+  ∃ T0, T = T0.weaken_var ∧ BoundVar Γ x T0 := by
+  intro he1 he2 h
+  cases h <;> try (solve | cases he1 | cases he2)
+  cases he1
+  simp [Fin.succ_inj] at he2
+  subst_vars
+  aesop
+
+def BoundVar.pred
+  {Γ : Ctx n m} {P : CType n m} {T : CType n.succ m} :
+  BoundVar (Ctx.extend_var Γ P) x.succ T ->
+  ∃ T0, T = T0.weaken_var ∧ BoundVar Γ x T0 := by
+  intro h
+  apply BoundVar.pred' <;> aesop
