CC/Narrowing.lean
@@ -1,0 +1,49 @@
+import Mathlib.Data.Finset.Basic
+import Mathlib.Data.Finset.Image
+
+import CC.Basic
+import CC.Rename
+
+import CC.CaptureSet
+import CC.Context
+import CC.Type
+import CC.Subcapt
+import CC.Subcapt.Basic
+import CC.Subcapt.Rename
+import CC.Subtype
+import CC.Subtype.Rename
+import CC.Subtype.Basic
+import CC.Subst
+
+namespace CC
+
+def VarSubst.narrowing_var
+  (h : Subtype Γ T' T) :
+  VarSubst (Ctx.extend_var Γ T) (Ctx.extend_var Γ T') id := by
+  unfold VarSubst
+  intro x P hb
+  cases x using Fin.cases with
+  | H0 =>
+    simp
+    cases hb
+    apply Typed.sub
+    apply Typed.var_bound_type
+    constructor
+    apply Subtype.weaken_var
+    trivial
+  | Hs x0 =>
+    simp
+    let ⟨P0, he, hb0⟩ := BoundVar.pred hb
+    subst_vars
+    apply Typed.var_bound_type
+    constructor
+    trivial
+
+def TVarRename.narrowing_var :
+  TVarRename (Ctx.extend_var Γ T) (Ctx.extend_var Γ T') id id := by
+  unfold TVarRename
+  intros X S h
+  simp
+  cases h
+  constructor
+  trivial
